iris/SmodePte.v
@@ -12,8 +12,9 @@ Require Import SailStdpp.ConcurrencyInterface SailStdpp.ConcurrencyInterfaceBuil
 Require Import Riscv.rv64d_types Riscv.rv64d.
 Require Import RiscvModelBytes.
 Require Import SailStdpp.Base SailStdpp.TypeCasts SailStdpp.Values SailStdpp.MachineWord.
-Require Import RiscvLang RiscvPtsto RiscvExec RiscvTryStep.
+Require Import RiscvLang RiscvPtsto RiscvExec RiscvTryStep RiscvFetchExec.
 Require Import WpLoad ExecCommon.
+Require Import RiscvExtras.   (* pma_ok_aligned + the pmaCheck/split peel kit *)
 Local Open Scope Z_scope.
 Import Defs.
 
@@ -319,43 +320,59 @@ Lemma exec_read_pte_S (addr : mword 64) (region : PMA_Region) (w : bv 64) s :
   exec (read_pte (Physaddr addr) 8) s = Some (Ok w, s).
 Proof.
   intros HA Hord Hrange HR Hmatch Halign Hread Hc Hsig Hh Hdev Hbytes.
+  (* pmaCheck now answers a splitting plan; an aligned access's plan is
+     [pma_ok_aligned], and check_pma_with_pmp_priority is pmaCheck on the
+     success path (RiscvExtras). *)
+  assert (Hpma : exec (pmaCheck (Physaddr addr) 8 (Load PageTableEntry) PBMT_PMA false) s
+                 = Some (Ok pma_ok_aligned, s)).
+  { destruct region as [rbase rsize rattr rdtree].
+    pma_ok_peel Hmatch Hread (exec_is_mag_applicable_load_pte 8 s) Halign. }
+  assert (Hcp : exec (check_pma_with_pmp_priority (Load PageTableEntry) PBMT_PMA Supervisor
+                        (Physaddr addr) 8 false) s = Some (Ok pma_ok_aligned, s)).
+  { unfold check_pma_with_pmp_priority.
+    rewrite (exec_bind_Some _ _ _ _ _ Hpma). cbn match. apply exec_returnM. }
+  assert (Hmmio : exec (within_mmio_readable (Physaddr addr) 8) s = Some (false, s)).
+  { unfold within_mmio_readable. cbn [get_config_rvfi].
+    rewrite (exec_or_boolM_Some _ _ _ _ _ Hc). cbn match.
+    rewrite (exec_or_boolM_Some _ _ _ _ _ Hsig). cbn match.
+    rewrite (exec_and_boolM_Some _ _ _ _ _ Hh). cbn match. reflexivity. }
   assert (Hchk : exec (checked_mem_read (Load PageTableEntry) PBMT_PMA Supervisor (Physaddr addr) 8 false false false false)
                    s = Some (Ok (w, default_meta), s)).
-  { unfold checked_mem_read.
-    rewrite (exec_bind_Some _ _ _ _ _
-              (_ : exec (phys_access_check _ _ _ _ _ _) s = Some (None, s))).
-    2:{ unfold phys_access_check.
-        rewrite (exec_bind_Some _ _ _ _ _
-                   (exec_pmpCheck_supervisor_grant_load addr 8 s HA Hord Hrange HR)).
-        cbn match.
-        rewrite (exec_bind_Some _ _ _ _ _
-                   (_ : exec (pmaCheck (Physaddr addr) 8 (Load PageTableEntry) PBMT_PMA false) s
-                        = Some (None, s))).
-        2:{ unfold pmaCheck.
-            rewrite (exec_bind_Some _ _ _ _ _ (exec_read_reg pma_regions s)).
-            rewrite Hmatch.
-            destruct region as [rbase rsize rattr rdtree].
-            cbn [PMA_Region_attributes] in Hread |- *.
-            rewrite Halign. cbn [Riscv.rv64d.not negb].
-            rewrite (exec_bind_Some _ _ _ _ _ (exec_returnM None s)).
-            cbn match beta.
-            change (assert_exp' true "sys/mem.sail:105.61-105.62" >>=
-                    (fun _ : true = true => returnM (PMA_supports_pte_read (override_PMA rattr PBMT_PMA))))
-              with (returnM (PMA_supports_pte_read (override_PMA rattr PBMT_PMA)) : M bool).
-            rewrite (exec_bind_Some _ _ _ _ _ (exec_returnM _ s)).
-            rewrite Hread. cbn match.
-            apply exec_returnM. }
-        cbn match. apply exec_returnM. }
-    rewrite (exec_bind_Some _ _ _ _ _
-              (_ : exec (within_mmio_readable (Physaddr addr) 8) s = Some (false, s))).
-    2:{ unfold within_mmio_readable. cbn [get_config_rvfi].
-        rewrite (exec_or_boolM_Some _ _ _ _ _ Hc). cbn match.
-        rewrite (exec_or_boolM_Some _ _ _ _ _ Hsig). cbn match.
-        rewrite (exec_and_boolM_Some _ _ _ _ _ Hh). cbn match. reflexivity. }
-    rewrite (exec_bind_Some _ _ _ _ _ (_ : exec (read_kind_of_flags _ _ _) s = Some (rv64d_types.Read_plain, s))).
+  { unfold checked_mem_read. rewrite exec_catch_early_return.
+    rewrite (execR_liftR_seq _ _ _ _ _ Hcp). cbn beta. cbn match.
+    rewrite execR_bind. rewrite execR_returnR. cbn match beta.
+    rewrite pma_ok_aligned_splittable pma_ok_aligned_granule.
+    rewrite (execR_liftR_seq _ _ _ _ _ (exec_split_misaligned_unsplit addr 8 0 s)). cbn beta.
+    rewrite misaligned_order_1. cbn zeta.
+    rewrite (execR_liftR_seq _ _ _ _ _
+               (_ : exec (read_kind_of_flags false false false) s = Some (rv64d_types.Read_plain, s))).
     2:{ unfold read_kind_of_flags. apply exec_returnM. }
-    rewrite (exec_bind_Some _ _ _ _ _ (exec_read_ram_plain_8 addr w s Hdev Hbytes)).
-    apply exec_returnM. }
+    cbn beta.
+    match goal with |- context[Defs.bind (Defs.untilMT ?vs ?m ?c ?b) _] =>
+      assert (Hu : execR (Defs.untilMT vs m c b) s = Some (inr (w, true, 0), s)) end.
+    { eapply execR_untilMT_1; [ reflexivity | | apply execR_returnR_fwd ].
+      rewrite (execR_liftR_seq _ _ _ _ _ (exec_assert_exp'_true _ s)). cbn beta.
+      change (bits_of_physaddr (Physaddr addr)) with addr.
+      rewrite avi0_mul8.
+      rewrite (execR_liftR_seq _ _ _ _ _
+                 (exec_pmpCheck_supervisor_grant_load addr 8 s HA Hord Hrange HR)). cbn beta.
+      cbn match.
+      match goal with |- context[Defs.bind (Defs.bind0 ?a ?b) _] =>
+        assert (Hseq : execR (Defs.bind0 a b) s = Some (inr false, s)) end.
+      { rewrite execR_bind0. rewrite execR_returnR. cbn match.
+        rewrite execR_liftR. rewrite Hmmio. reflexivity. }
+      rewrite (execR_bind_Some _ _ _ _ _ Hseq). cbn beta. cbn match.
+      match goal with
+        |- context[Defs.bind (Defs.bind (Defs.liftR (read_ram ?rk ?pa ?wd ?mt)) ?k1) _] =>
+        assert (Hrd : execR (Defs.bind (Defs.liftR (read_ram rk pa wd mt)) k1) s
+                      = Some (inr w, s)) end.
+      { rewrite (execR_liftR_seq _ _ _ _ _ (exec_read_ram_plain_8 addr w s Hdev Hbytes)).
+        cbn beta match. apply execR_returnR_fwd. }
+      rewrite (execR_bind_Some _ _ _ _ _ Hrd). cbn beta zeta.
+      rewrite autocast_id. rewrite usvd_zeros_full_64.
+      apply execR_returnR_fwd. }
+    rewrite (execR_bind_Some _ _ _ _ _ Hu). cbn beta zeta.
+    rewrite autocast_id. rewrite execR_returnR. reflexivity. }
   unfold read_pte, mem_read_priv.
   rewrite (exec_bind_Some _ _ _ _ _
             (_ : exec (mem_read_priv_meta _ _ _ _ 8 _ _ _ _) s = Some (Ok (w, default_meta), s))).
