iris/WpMmodeLeafBase.v
@@ -402,7 +402,10 @@ Proof.
   rewrite (execR_bind_Some _ _ _ _ _ (execR_returnR_fwd (Virtaddr a8) s)).
   rewrite execR_liftR.
   rewrite (exec_vmem_read_addr_8 a8 v region s Halign Hcp Hmprv Hpmp Hmatch Hpalign Hread Hc Hsig Hh Hdev Hbytes).
-  reflexivity.
+  (* the vmem lemma hands back the value itself now: the split loop's
+     full-width accumulator write is discharged there (usvd_zeros_full_64) *)
+  change data2 with (update_subrange_vec_dec (zeros' (8*1*8)) (8*(0+1)*8-1) (8*0*8) v).
+  rewrite usvd_zeros_full_64. reflexivity.
 Qed.
 End VRg.
 
@@ -541,27 +544,52 @@ Lemma exec_checked_mem_write_ram_store (pbmt : page_based_mem_type) (addr : mwor
     = Some (Ok true, MState s.(sregs) (write_bytes s.(mem) addr 8 data) s.(mdev)).
 Proof.
   intros Hpmp Hmatch Halign Hwrite Hc Hsig Hh Hdev.
-  unfold checked_mem_write.
-  rewrite (exec_bind_Some _ _ _ _ _
-            (_ : exec (phys_access_check _ _ _ _ _ _) s = Some (None, s))).
-  2:{ unfold phys_access_check.
-      rewrite (exec_bind_Some _ _ _ _ _ (exec_pmpCheck_machine_none _ _ _ s Hpmp)).
-      cbn match.
-      rewrite (exec_bind_Some _ _ _ _ _ (exec_pmaCheck_ram_store addr pbmt region s Hmatch Halign Hwrite)).
-      cbn match. apply exec_returnM. }
-  cbn match.
-  rewrite (exec_bind_Some _ _ _ _ _
-            (_ : exec (within_mmio_writable (Physaddr addr) 8) s = Some (false, s))).
-  2:{ unfold within_mmio_writable. cbn [get_config_rvfi].
-      rewrite (exec_or_boolM_Some _ _ _ _ _ Hc). cbn match.
-      rewrite (exec_or_boolM_Some _ _ _ _ _ Hsig). cbn match.
-      rewrite (exec_and_boolM_Some _ _ _ _ _ Hh). cbn match. reflexivity. }
-  cbn match.
-  rewrite (exec_bind_Some _ _ _ _ _
-            (_ : exec (write_kind_of_flags false false false) s = Some (rv64d_types.Write_plain, s))).
+  assert (Hcp : exec (check_pma_with_pmp_priority (Store Data) pbmt Machine
+                        (Physaddr addr) 8 false) s = Some (Ok pma_ok_aligned, s)).
+  { unfold check_pma_with_pmp_priority.
+    rewrite (exec_bind_Some _ _ _ _ _
+               (exec_pmaCheck_ram_store addr pbmt region s Hmatch Halign Hwrite)).
+    cbn match. apply exec_returnM. }
+  assert (Hmmio : exec (within_mmio_writable (Physaddr addr) 8) s = Some (false, s)).
+  { unfold within_mmio_writable. cbn [get_config_rvfi].
+    rewrite (exec_or_boolM_Some _ _ _ _ _ Hc). cbn match.
+    rewrite (exec_or_boolM_Some _ _ _ _ _ Hsig). cbn match.
+    rewrite (exec_and_boolM_Some _ _ _ _ _ Hh). cbn match. reflexivity. }
+  set (sw := MState s.(sregs) (write_bytes s.(mem) addr 8 data) s.(mdev)).
+  unfold checked_mem_write. rewrite exec_catch_early_return.
+  rewrite (execR_liftR_seq _ _ _ _ _ Hcp). cbn beta. cbn match.
+  rewrite execR_bind. rewrite execR_returnR. cbn match beta.
+  rewrite pma_ok_aligned_splittable pma_ok_aligned_granule.
+  rewrite (execR_liftR_seq _ _ _ _ _ (exec_split_misaligned_unsplit addr 8 0 s)). cbn beta.
+  rewrite misaligned_order_1. cbn zeta.
+  rewrite (execR_liftR_seq _ _ _ _ _
+             (_ : exec (write_kind_of_flags false false false) s
+                  = Some (rv64d_types.Write_plain, s))).
   2:{ unfold write_kind_of_flags. cbn match. apply exec_returnM. }
-  rewrite (exec_bind_Some _ _ _ _ _ (exec_write_ram_plain_8 addr data s Hdev)).
-  apply exec_returnM.
+  cbn beta.
+  (* one split, at offset 0 *)
+  match goal with |- context[Defs.bind (Defs.untilMT ?vs ?m ?c ?b) _] =>
+    assert (Hu : execR (Defs.untilMT vs m c b) s = Some (inr (true, 0, true), sw)) end.
+  { eapply execR_untilMT_1; [ reflexivity | | apply execR_returnR_fwd ].
+    rewrite (execR_liftR_seq _ _ _ _ _ (exec_assert_exp'_true _ s)). cbn beta.
+    change (bits_of_physaddr (Physaddr addr)) with addr.
+    rewrite avi0_mul8.
+    rewrite (execR_liftR_seq _ _ _ _ _ (exec_pmpCheck_machine_none _ _ _ s Hpmp)). cbn beta.
+    cbn match.
+    match goal with |- context[Defs.bind (Defs.bind0 ?a ?b) _] =>
+      assert (Hseq : execR (Defs.bind0 a b) s = Some (inr false, s)) end.
+    { rewrite execR_bind0. rewrite execR_returnR. cbn match.
+      rewrite execR_liftR. rewrite Hmmio. reflexivity. }
+    rewrite (execR_bind_Some _ _ _ _ _ Hseq). cbn beta. cbn match.
+    (* the split's value is the full-width subrange of the data, i.e. the data *)
+    rewrite autocast_id.
+    change (8 * (0 + 1) * 8 - 1) with 63. change (8 * 0 * 8) with 0.
+    rewrite subrange_full_64.
+    rewrite (execR_liftR_seq _ _ _ _ _ (exec_write_ram_plain_8 addr data s Hdev)).
+    cbn beta zeta. cbn [andb].
+    apply execR_returnR_fwd. }
+  rewrite (execR_bind_Some _ _ _ _ _ Hu). cbn beta zeta.
+  rewrite execR_returnR. reflexivity.
 Qed.
 
 (* WpGprStore.v : exec_effectivePrivilege_store *)
